---

### Equation (a)

$$
z^2 + (1 - 5i)z + (2i - 6) = 0
$$

* $a = 1$, $b = 1 - 5i$, $c = 2i - 6$

$$
D = b^2 - 4ac = (1 - 5i)^2 - 4(1)(2i - 6)
$$

$$
(1 - 5i)^2 = 1 - 10i + 25i^2 = 1 - 10i - 25 = -24 - 10i
$$

$$
-4(2i - 6) = -8i + 24
$$

$$
D = (-24 - 10i) + (24 - 8i) = -18i
$$

---

### Equation (b)

$$
z^2 - (3 + 4i)z + (7i - 1) = 0
$$

* $a = 1$, $b = -(3 + 4i)$, $c = 7i - 1$

$$
D = b^2 - 4ac = [-(3 + 4i)]^2 - 4(7i - 1)
$$

$$
(-(3 + 4i))^2 = (-(3 + 4i)) \cdot (-(3 + 4i)) = (3 + 4i)^2
$$

$$
(3 + 4i)^2 = 9 + 24i + 16i^2 = 9 + 24i - 16 = -7 + 24i
$$

$$
-4(7i - 1) = -28i + 4
$$

$$
D = (-7 + 24i) + (4 - 28i) = -3 - 4i
$$

---

### Equation (c)

$$
2z^2 + (5 + i)z + (2 + 2i) = 0
$$

* $a = 2$, $b = 5 + i$, $c = 2 + 2i$

$$
D = b^2 - 4ac = (5 + i)^2 - 4(2)(2 + 2i)
$$

$$
(5 + i)^2 = 25 + 10i + i^2 = 25 + 10i - 1 = 24 + 10i
$$

$$
4 \cdot 2 \cdot (2 + 2i) = 16 + 16i
$$

$$
D = (24 + 10i) - (16 + 16i) = 8 - 6i
$$

---

### Final Table

  <table>
    <thead>
      <tr>
        <th>Equation</th>
        <th>Discriminant <code>D = b² − 4ac</code></th>
      </tr>
    </thead>
    <tbody>
      <tr>
        <td><code>z<sup>2</sup> + (1 − 5i)z + 2i − 6 = 0</code></td>
        <td><code>−18i</code></td>
      </tr>
      <tr>
        <td><code>z<sup>2</sup> − (3 + 4i)z + 7i − 1 = 0</code></td>
        <td><code>−3 − 4i</code></td>
      </tr>
      <tr>
        <td><code>2z<sup>2</sup> + (5 + i)z + 2 + 2i = 0</code></td>
        <td><code>8 − 6i</code></td>
      </tr>
    </tbody>
  </table>

