
## Formule quadratique

$$
z=\frac{-b\pm\sqrt{D}}{2a},\qquad D=b^2-4ac.
$$

---

### (a) $z^2+(1-5i)z+(2i-6)=0$

$a=1,\; b=1-5i,\; c=2i-6.$
On a trouvé $D=-18i.$

On cherche $\sqrt{D}=\sqrt{-18i}$.

$$
\sqrt{D}=\pm(3-3i).
$$

Formule quadratique :

$$
z=\frac{-(1-5i)\pm(3-3i)}{2}
=\frac{-1+5i\pm(3-3i)}{2}.
$$

* Avec le « + » : $(2+2i)/2=1+i$.
* Avec le « – » : $(-4+8i)/2=-2+4i$.

**Racines (a) :** $\boxed{1+i,\; -2+4i}$.

---

### (b) $z^2-(3+4i)z+(7i-1)=0$

$a=1,\; b=-3-4i,\; c=7i-1.$
On a trouvé $D=-3-4i.$

On cherche $\sqrt{D}=\sqrt{-3-4i}$.

$$
\sqrt{D}=\pm(1-2i).
$$

Formule quadratique :

$$
z=\frac{-b\pm\sqrt{D}}{2}=\frac{3+4i\pm(1-2i)}{2}.
$$

* Avec le « + » : $(4+2i)/2=2+i$.
* Avec le « – » : $(2+6i)/2=1+3i$.

**Racines (b) :** $\boxed{2+i,\; 1+3i}$.

---

### (c) $2z^2+(5+i)z+(2+2i)=0$

$a=2,\; b=5+i,\; c=2+2i.$
On a trouvé $D=8-6i.$

On cherche $\sqrt{D}=\sqrt{8-6i}$.

$$
\sqrt{D}=\pm(3-i).
$$

Formule quadratique ($2a=4$) :

$$
z=\frac{-(5+i)\pm(3-i)}{4}.
$$

* Avec le « + » : $(-2-2i)/4=-\tfrac{1+i}{2}$.
* Avec le « – » : $(-8)/4=-2$.

**Racines (c) :** $\boxed{-2,\; -\tfrac{1+i}{2}}$.

---

## Résumé — toutes les racines

* (a) $1+i,\; -2+4i$
* (b) $2+i,\; 1+3i$
* (c) $-2,\; -\dfrac{1+i}{2}$



