
### a) $(1 - i)^2$

$$
(1 - i)^2 = (1 - i)(1 - i)
$$

$$
= 1 \cdot 1 - 1 \cdot i - i \cdot 1 + i^2
$$

$$
= 1 - i - i + (-1)
$$

$$
= (1 - 1) - 2i = -2i
$$

✅ **Result:** $-2i$

---

### c) $(2 + 3i)^2$

$$
(2 + 3i)^2 = (2 + 3i)(2 + 3i)
$$

$$
= 2\cdot 2 + 2 \cdot 3i + 3i \cdot 2 + (3i)^2
$$

$$
= 4 + 6i + 6i + 9i^2
$$

$$
= 4 + 12i + 9(-1)
$$

$$
= 4 + 12i - 9
$$

$$
= -5 + 12i
$$

✅ **Result:** $-5 + 12i$

---

### e) $(2 - i)(3 - 4i)$

$$
(2 - i)(3 - 4i) = 2 \cdot 3 + 2 \cdot (-4i) + (-i)\cdot 3 + (-i)(-4i)
$$

$$
= 6 - 8i - 3i + 4i^2
$$

$$
= 6 - 11i + 4(-1)
$$

$$
= 6 - 11i - 4
$$

$$
= 2 - 11i
$$

✅ **Result:** $2 - 11i$

---

✨ Final Answers:

* a) $-2i$
* c) $-5 + 12i$
* e) $2 - 11i$


